asgin 12 done

sf/Assignment12_05.v
@@ -13,31 +13,90 @@ Require Export Assignment12_04.
 *)
 
 Definition halve : tm :=
-  FILL_IN_HERE.
+  tfix
+  (tabs K (TArrow TNat TNat) 
+    (tabs N TNat (tif0 (tvar N) (tnat 0)
+                   (tif0 (tpred (tvar N)) (tnat 0)
+                     (tsucc (tapp (tvar K) (tpred (tpred (tvar N))))))))).
 
 Example halve_type: empty |- halve \in TArrow TNat TNat.
 Proof.
-  (* unfold halve; eauto 10. *)
-  exact FILL_IN_HERE.
+  unfold halve; eauto 10.
 Qed.
 
 Example halve_10: tapp halve (tnat 10) ==>* tnat 5.
 Proof.
-  (* unfold halve; normalize. *)
-  exact FILL_IN_HERE.
+  unfold halve; normalize.
 Qed.
 
 Example halve_11: tapp halve (tnat 11) ==>* tnat 5.
 Proof.
-  (* unfold halve; normalize. *)
-  exact FILL_IN_HERE.
+  unfold halve; normalize.
 Qed.
 
 
 Theorem halve_correct: forall n,
    tapp halve (tnat (n+n)) ==>* tnat n.
 Proof.
-  exact FILL_IN_HERE.
+  induction n.
+  simpl.
+  eapply multi_step.
+  apply ST_AppFix.
+  eauto. eauto.
+  eapply multi_step.
+  apply ST_App1.
+  apply ST_AppAbs.
+  eauto.
+  simpl.
+  eapply multi_step.
+  apply ST_AppAbs.
+  eauto.
+  eapply multi_step.
+  simpl.
+  apply ST_If0Zero. eauto.
+  replace (S n + S n) with (S (S (n + n))); try omega.
+  eapply multi_step.
+  apply ST_AppFix; eauto.
+  eapply multi_step.
+  apply ST_App1.
+  apply ST_AppAbs.
+  eauto.
+  simpl.
+  eapply multi_step.
+  apply ST_AppAbs.
+  eauto.
+  simpl.
+  eapply multi_step.
+  apply ST_If0Nonzero.
+  eapply multi_step.
+  apply ST_If01.
+  apply ST_PredNat.
+  eapply multi_step.
+  simpl.
+  apply ST_If0Nonzero.
+  eapply multi_step.
+  apply ST_Succ1.
+  apply ST_App2.
+  eauto.
+  apply ST_Pred.
+  apply ST_PredNat.
+  eapply multi_step.
+  apply ST_Succ1.
+  simpl.
+  apply ST_App2.
+  eauto.
+  apply ST_PredNat.
+  simpl.
+  assert (forall t t', t ==>* t' -> tsucc t ==>* tsucc t').
+  intros. induction H. constructor.
+  eapply multi_step.
+  apply ST_Succ1.
+  apply H. assumption.
+  eapply multi_trans.
+  apply H. apply IHn.
+  eapply multi_step.
+  apply ST_SuccNat.
+  constructor.
 Qed.
 
 (*-- Check --*)
