sf/Assignment12_06.v
@@ -1,11 +1,123 @@
 Require Export Assignment12_05.
 
-(* problem #06: 10 points *)
+(* problem #06: 10 points *)  
+
+Notation FA := (tapp tloop (tnat 0)).
+Notation FB := (
+tapp
+  (tapp
+     (tabs Loop (TArrow TNat TNat) (tabs X TNat (tapp (tvar Loop) (tvar X))))
+     (tfix
+        (tabs Loop (TArrow TNat TNat)
+           (tabs X TNat (tapp (tvar Loop) (tvar X)))))) (tnat 0)).
+Notation FC := (tapp
+  ([Loop
+   := tfix
+        (tabs Loop (TArrow TNat TNat)
+           (tabs X TNat (tapp (tvar Loop) (tvar X))))]
+   tabs X TNat (tapp (tvar Loop) (tvar X))) (tnat 0)
+).
+
+Lemma AB : FA ==> FB.
+Proof.
+apply ST_AppFix; eauto. Qed.
+Lemma BC : FB ==> FC.
+Proof.
+apply ST_App1; eauto. Qed.
+Lemma CA : FC ==> FA.
+Proof.
+apply ST_AppAbs;eauto. Qed.
+
+Inductive nstep : tm -> nat -> tm -> Prop :=
+| nstep0 : forall S, nstep S 0 S 
+| nstepS : forall T TT TTT n,
+   T ==> TT -> nstep TT n TTT -> nstep T (S n) TTT.
+
+Lemma multi_n :
+forall t t1, t ==>* t1 -> exists n, nstep t n t1.
+Proof.
+intros.
+induction H. exists 0; constructor.
+inversion IHmulti as [n p]. exists (S n).
+eapply nstepS. apply H. assumption. Qed.
+
+Lemma A_B:
+forall t, FA ==> t -> t = FB.
+Proof.
+  intros.
+  inversion H;subst;try auto.
+  inversion H3;subst.
+  inversion H1;subst.
+  inversion H4.
+Qed.
+
+Lemma B_C:
+forall t, FB ==> t -> t = FC.
+Proof.
+  intros.
+  inversion H;subst;auto.
+  inversion H3;subst.
+  auto.
+  inversion H4;subst.
+  inversion H5;subst.
+  inversion H1;subst.
+  inversion H4.
+Qed.
+
+Lemma C_A:
+forall t, FC ==> t -> t = FA.
+Proof.
+  intros.
+  inversion H; subst; try auto.
+  inversion H3;subst; try auto.
+  inversion H4.
+Qed.
+
+Lemma ABC_n :
+forall n t, nstep FA n t \/ nstep FB n t \/ nstep FC n t
+-> t = FA \/ t = FB \/ t = FC.
+Proof.
+induction n; intros. 
+inversion H as [P | [P | P]];
+inversion P;subst;auto.
+inversion H as [P | [P | P]].
+inversion P; subst. apply A_B in H1. subst.
+assert (nstep FA n t \/ nstep FB n t \/ nstep FC n t). auto.
+apply IHn in H0. auto.
+inversion P; subst. apply B_C in H1; subst.
+assert (nstep FA n t \/ nstep FB n t \/ nstep FC n t). auto.
+apply IHn in H0. auto.
+inversion P; subst. apply C_A in H1; subst.
+assert (nstep FA n t \/ nstep FB n t \/ nstep FC n t). auto.
+apply IHn in H0. auto.
+Qed.
+
+
+Lemma ABC :
+forall t, FA ==>* t -> t = FA \/ t = FB \/ t = FC.
+Proof.
+  intros.
+  assert (HH := multi_n FA t).
+  apply HH in H.
+  inversion H.
+  assert (nstep FA x t \/ nstep FB x t \/ nstep FC x t). auto.
+  apply ABC_n in H1. auto.
+Qed.
 
 Theorem tloop_diverges:
   ~ exists t, tapp tloop (tnat 0) ==>* t /\ normal_form step t.
 Proof.
-  exact FILL_IN_HERE.
+  unfold not. intros.
+  inversion H.
+  destruct H0. clear H.
+  unfold normal_form in H1.
+  unfold not in H1.
+  apply ABC in H0.
+  apply H1.
+  inversion H0 as [X | [Y | Z]].
+  exists FB. rewrite X. apply AB.
+  exists FC. rewrite Y. apply BC.
+  exists FA. rewrite Z. apply CA.
 Qed.
 
 (*-- Check --*)
