sf/Assignment12_01.v
@@ -8,6 +8,16 @@ Require Export Assignment12_00.
           empty |- \x:S. x x : T).
 *)
 
+Lemma stupid:
+  forall T1 T2, ~ T1 = TArrow T1 T2.
+Proof.
+  unfold not.
+  intros.
+  generalize dependent T2.
+  induction T1; intros; inversion H.
+  apply IHT1_1 in H1; assumption.
+Qed.
+
 Example typing_nonexample_3 :
   ~ (exists S, exists T,
         empty |- 
@@ -15,7 +25,19 @@ Example typing_nonexample_3 :
              (tapp (tvar X) (tvar X))) \in
           T).
 Proof.
-  exact FILL_IN_HERE.
+  unfold not; intros.
+  inversion H as [S [T p]].
+  inversion p; subst.
+  inversion H5;subst.
+  inversion H6;subst.
+  unfold extend in H2.
+  simpl in H2.
+  inversion H2;subst.
+  inversion H3;subst.
+  unfold extend in H4.
+  simpl in H4.
+  inversion H4.
+  apply stupid in H1;assumption.
 Qed.
 
 (*-- Check --*)
