sf/Assignment12_03.v
@@ -12,7 +12,18 @@ Lemma type_is_unique: forall t G T T'
     (TYPED': G |- t \in T'),
   T = T'.
 Proof.
-  exact FILL_IN_HERE.
+  intros.
+  generalize dependent T'.
+  induction TYPED; intros; try (inversion TYPED'; auto);
+  try (apply IHTYPED in H1; inversion H1; auto).
+  inversion TYPED'; subst. rewrite H in H2; inversion H2; auto.
+  inversion TYPED'; subst. apply IHTYPED in H4. rewrite H4; auto.
+  inversion TYPED';subst. apply IHTYPED1 in H2; apply IHTYPED2 in H4;inversion H2;auto.
+  apply IHTYPED1 in H2; apply IHTYPED2 in H4; subst; auto.
+  apply IHTYPED1 in H4. inversion TYPED'; subst. apply IHTYPED2 in H5. auto.
+  apply IHTYPED in H3. rewrite H3. auto.
+  apply IHTYPED in H3. rewrite H3; auto.
+  apply IHTYPED1 in H6. inversion H6. subst. auto.
 Qed.
 
 (*-- Check --*)
