sf/Assignment12_04.v
@@ -7,7 +7,15 @@ Corollary soundness : forall t t' T,
   t ==>* t' ->
   ~(stuck t').
 Proof.
-  exact FILL_IN_HERE.
+  unfold not. unfold stuck. unfold not. intros.
+  destruct H1.
+  unfold normal_form in H1.
+  unfold not in H1.
+  induction H0.
+  apply progress in H.
+  inversion H. apply H2 in H0;auto. apply H1 in H0;auto.
+  eapply preservation in H; (try apply H0).
+  apply IHmulti in H; try assumption.
 Qed.
 
 (*-- Check --*)
